\documentclass{article}

\usepackage[hscale=0.7,vscale=0.8]{geometry}

%\usepackage{lipsum}

\pagenumbering{gobble}

\begin{document}

\textbf{Area of Rectangle}
\begin{equation}
Area_{\;rectangle} = width * height
\end{equation}

\textbf{Perimeter of a Rectangle}
Is the sum of the 4 sides
\begin{equation}
Perimeter_{\;Rectangle} = 2 ( width + height )
\end{equation}

\textbf{Angles of a Four sided figure}
\begin{equation}
Sum\;of\;Angles\;of\;any\;Four\; sided\; figure = 360^\circ
\end{equation}


\textbf{Angles of a Triangle}
\begin{equation}
Sum\;of\;Angles\;of\;a\;Triangle = 180^\circ
\end{equation}


\textbf{Area of a Triangle}
\begin{equation}
Area_{Triangle} = \frac{base}{2} * Perpindicular Height
\end{equation}

\textbf{Pythagoras Theorem}
\begin{equation}
h^2 = a^2 + b^2 \;\;so \;\;h= \sqrt{a^2 + b^2}
\end{equation}

\textbf{Circles}

\textit{Area of a Circle}
\begin{equation}
Area_{ Circle} = \pi r^ 2
\end{equation}

\textit{Circumference of a Circle}
\begin{equation}
Circumference_{ Circle} = 2 \pi r
\end{equation}

\textbf{Sectors of a Circle}

\textit{Area of a Sector of a Circle}
\begin{equation}
Area_{ Sector\;of\;a\;Circle} = ( \frac{Angle }{ 360 }) \pi r^ 2
\end{equation}


\textit{Circumference of a Sector of a Circle}
\begin{equation}
Circumference_{ Sector\;of\;a\;Circle} = ( \frac{Angle }{ 360} ) 2 \pi r
\end{equation}


\textbf{Rectangular Box}
\begin{equation}
Volume_{box} = width * height * depth
\end{equation}

\begin{equation}
Surface\;Area_{box} = 2(width * height) + 2(width * depth) + 2(height * depth)
\end{equation}

\textbf{Cylinder}
\begin{equation}
Volume_{ Cylinder} = h \pi r^ 2
\end{equation}

\begin{equation}
Surface\;Area_{ Cylinder} = 2 \pi r h + 2(\pi r^ 2 )
\end{equation}

\textbf{Slope of a Line}

\textit{Using the Equation}
\begin{equation}
y = mx + B
\end{equation}

\textit{Using Co-ordinates ($x_1$, $y_1$) and ($x_2$, $y_2$) }
\begin{equation}
m = \frac{ (y_2 - y_1) }{ (x_2 - y_1) }
\end{equation}

\textbf{Length of a Line with co-ordinates  ($x_1$, $y_1$) and ($x_2$, $y_2$) }
\begin{equation}
h= \sqrt{(x_{2}-x_{1})^2 + (y_{2}-y_{1})^2}
\end{equation}


\end{document}